Add the shallow embedded version of i2c_core
Three contributions of this commit:

1. The shallow embedded model/version of `i2c_core`
2. The script to generate its corresponding verilog equivalent together
   with its proof
3. Specialise the i2c_reg_top proof for i2c_circuit

i2c/i2cCoreCircuitLib.sml
@@ -1,0 +1,579 @@
+structure i2cCoreCircuitLib =
+struct
+
+open wordsLib;
+open i2cCircuitStateTheory i2cRegsTheory i2cRegsCommTheory;
+open i2cCoreTheory;
+
+Overload idle = “0w : 5 word”;
+Overload active = “1w : 5 word”;
+Overload recReadClockLow = “2w : 5 word”;
+Overload recReadClockPulse = “3w : 5 word”;
+Overload recReadHoldBit = “4w : 5 word”;
+Overload recHostClockLowAck = “5w : 5 word”;
+Overload recHostClockPulseAck = “6w : 5 word”;
+Overload recHostHoldBitAck = “7w : 5 word”;
+Overload stopClockStop = “8w : 5 word”;
+Overload stopSetupStop = “9w : 5 word”;
+Overload stopHoldStop = “10w : 5 word”;
+Overload startSetupStart = “11w : 5 word”;
+Overload startHoldStart = “12w : 5 word”;
+Overload startClockStart = “13w : 5 word”;
+Overload transClockLow = “14w : 5 word”;
+Overload transClockPulse = “15w : 5 word”;
+Overload transHoldBit = “16w : 5 word”;
+Overload transClockLowAck = “17w : 5 word”;
+Overload transClockPulseAck = “18w : 5 word”;
+Overload transHoldDevAck = “19w : 5 word”;
+Overload popFmtFifo = “20w : 5 word”;
+
+(* soft reset *)
+val fmt_fifo_reset_tm = “
+ s' with fmt_fifo := s'.fmt_fifo with reset := ((s'.reg2hw.fifo_ctrl.fmtrst_q = 1w) ∧ s.reg2hw.fifo_ctrl.fmtrst_qe)
+”;
+
+(* Reading register file via read pointer *)
+val fmt_fifo_rdata_tm = “
+ s' with fmt_fifo := s'.fmt_fifo with rdata := s.fmt_fifo_regfile $ (5 >< 0) s.fmt_fifo.rptr
+”;
+
+(* Section --- Updating read pointer *)
+val fmt_fifo_rready_tm = “
+ s' with fmt_fifo := s'.fmt_fifo with rready := (s.fsm_state = popFmtFifo)
+”;
+
+val fmt_fifo_empty_tm = “
+ s' with fmt_fifo := s'.fmt_fifo with empty := (s.fmt_fifo.rptr = s.fmt_fifo.wptr)
+”;
+
+val fmt_fifo_incr_rptr_tm = “
+ s' with fmt_fifo := s'.fmt_fifo with incr_rptr := (¬s'.fmt_fifo.empty ∧ s'.fmt_fifo.rready)
+”;
+
+val fmt_fifo_counter_rptr_wrap_tm = “
+ s' with fmt_fifo := s'.fmt_fifo with counter2 := s'.fmt_fifo.counter2 with rptr_wrap :=
+   (s'.fmt_fifo.incr_rptr ∧ (5 >< 0) s.fmt_fifo.rptr = 63w : 6 word)
+”;
+
+val fmt_fifo_counter_rptr_wrap_cnt_tm = “
+ s' with fmt_fifo := s'.fmt_fifo with counter2 := s'.fmt_fifo.counter2 with rptr_wrap_cnt :=
+  if ¬ word_bit 6 s.fmt_fifo.rptr then (64w : 7 word) else 0w
+”;
+
+val fmt_fifo_rptr_tm = “
+ if s'.fmt_fifo.reset then
+   s' with fmt_fifo := s'.fmt_fifo with rptr := 0w
+ else if s'.fmt_fifo.counter2.rptr_wrap then
+   s' with fmt_fifo := s'.fmt_fifo with rptr := s'.fmt_fifo.counter2.rptr_wrap_cnt
+ else
+   s' with fmt_fifo := s'.fmt_fifo with rptr := s.fmt_fifo.rptr + 1w
+”;
+
+(* Updating register file via write pointer *)
+val fmt_fifo_wvalid_tm = “
+   s' with fmt_fifo := s'.fmt_fifo with wvalid :=
+   (s.reg2hw.fdata.fbyte_qe ∧ s.reg2hw.fdata.start_qe ∧ s.reg2hw.fdata.stop_qe ∧ s.reg2hw.fdata.read_qe ∧ s.reg2hw.fdata.rcont_qe ∧ s.reg2hw.fdata.nakok_qe)
+”;
+
+val fmt_fifo_full_tm = “
+ s' with fmt_fifo := s'.fmt_fifo with full :=
+ ( word_bit 6 s.fmt_fifo.wptr ≠ word_bit 6 s.fmt_fifo.rptr
+ ∧ (5 >< 0) s.fmt_fifo.wptr : 6 word = (5 >< 0) s.fmt_fifo.rptr : 6 word)
+”;
+
+val fmt_fifo_incr_wptr_tm = “
+ s' with fmt_fifo := s'.fmt_fifo with incr_wptr := (¬s'.fmt_fifo.full ∧ s'.fmt_fifo.wvalid)
+”;
+
+val fmt_fifo_wdata_tm = “
+   s' with fmt_fifo := s'.fmt_fifo with wdata :=
+           	      (w2w s'.reg2hw.fdata.nakok_q <<~ 12w)
+                   || (w2w s'.reg2hw.fdata.rcont_q <<~ 11w)
+                   || (w2w s'.reg2hw.fdata.read_q <<~ 10w)
+                   || (w2w s'.reg2hw.fdata.stop_q <<~ 9w)
+                   || (w2w s'.reg2hw.fdata.start_q <<~ 8w)
+                   ||  w2w s'.reg2hw.fdata.fbyte_q
+”;
+
+val fmt_fifo_regfile_tm = “
+ let
+   wptr = (5 >< 0) s.fmt_fifo.wptr;
+ in
+   if s'.fmt_fifo.incr_wptr
+   then s' with fmt_fifo_regfile := (wptr =+ s'.fmt_fifo.wdata) s'.fmt_fifo_regfile
+   else s'
+”;
+
+(* Section --- updating the write pointer *)
+val fmt_fifo_counter_wptr_wrap_tm = “
+ s' with fmt_fifo := s'.fmt_fifo with counter2 := s'.fmt_fifo.counter2 with wptr_wrap :=
+   (s'.fmt_fifo.incr_wptr ∧ (5 >< 0) s.fmt_fifo.wptr = 63w : 6 word)
+”;
+
+val fmt_fifo_counter_wptr_wrap_cnt_tm = “
+ s' with fmt_fifo := s'.fmt_fifo with counter2 := s'.fmt_fifo.counter2 with wptr_wrap_cnt :=
+    if ¬ (word_bit 6 s.fmt_fifo.wptr) then 64w else 0w
+”;
+
+val fmt_fifo_wptr_tm = “
+ if s'.fmt_fifo.reset then
+   s' with fmt_fifo := s'.fmt_fifo with wptr := 0w
+ else if s'.fmt_fifo.counter2.wptr_wrap then
+   s' with fmt_fifo := s'.fmt_fifo with wptr := s'.fmt_fifo.counter2.wptr_wrap_cnt
+ else
+   s' with fmt_fifo := s'.fmt_fifo with wptr := s.fmt_fifo.wptr + 1w
+”;
+
+(* section --- Finite State Machine *)
+val delay_tm = “
+ let
+   s' = s' with delay := s'.delay with setup_start := w2w s.regs.timing1.t_r + w2w s.regs.timing2.tsu_sta ;
+   s' = s' with delay := s'.delay with hold_start  := w2w s.regs.timing1.t_f + w2w s.regs.timing2.thd_sta ;
+   s' = s' with delay := s'.delay with setup_data  := w2w s.regs.timing1.t_r + w2w s.regs.timing3.tsu_dat ;
+   s' = s' with delay := s'.delay with clock_start := w2w s.regs.timing3.thd_dat ;
+   s' = s' with delay := s'.delay with clock_low   := w2w s.regs.timing0.tlow - w2w s.regs.timing3.thd_dat;
+   s' = s' with delay := s'.delay with clock_pulse := w2w s.regs.timing1.t_r + w2w s.regs.timing0.thigh + w2w s.regs.timing1.t_f ;
+   s' = s' with delay := s'.delay with hold_bit    := w2w s.regs.timing1.t_f + w2w s.regs.timing3.thd_dat ;
+   s' = s' with delay := s'.delay with clock_stop  := w2w s.regs.timing1.t_f + w2w s.regs.timing0.tlow - w2w s.regs.timing3.thd_dat ;
+   s' = s' with delay := s'.delay with setup_stop  := w2w s.regs.timing1.t_r + w2w s.regs.timing4.tsu_sto ;
+   s' = s' with delay := s'.delay with hold_stop   := w2w s.regs.timing1.t_r + w2w s.regs.timing4.t_buf - w2w s.regs.timing2.tsu_sta ;
+ in
+   s'
+”;
+
+val curr_delay_tm = “
+ case s.fsm_state of
+   recReadClockLow      => s' with curr_delay := s'.delay.clock_low
+ | recReadClockPulse    => s' with curr_delay := s'.delay.clock_pulse
+ | recReadHoldBit       => s' with curr_delay := s'.delay.hold_bit
+ | recHostClockLowAck   => s' with curr_delay := s'.delay.clock_low
+ | recHostClockPulseAck => s' with curr_delay := s'.delay.clock_pulse
+ | recHostHoldBitAck    => s' with curr_delay := s'.delay.hold_bit
+ | stopClockStop        => s' with curr_delay := s'.delay.clock_stop
+ | stopSetupStop        => s' with curr_delay := s'.delay.setup_stop
+ | stopHoldStop         => s' with curr_delay := s'.delay.hold_stop
+ | startSetupStart      => s' with curr_delay := s'.delay.setup_start
+ | startHoldStart       => s' with curr_delay := s'.delay.hold_start
+ | startClockStart      => s' with curr_delay := s'.delay.clock_start
+ | transClockLow        => s' with curr_delay := s'.delay.clock_low
+ | transClockPulse      => s' with curr_delay := s'.delay.clock_pulse
+ | transHoldBit         => s' with curr_delay := s'.delay.hold_bit
+ | transClockLowAck     => s' with curr_delay := s'.delay.clock_low
+ | transClockPulseAck   => s' with curr_delay := s'.delay.clock_pulse
+ | transHoldDevAck      => s' with curr_delay := s'.delay.hold_bit
+ | _                    => s' with curr_delay := 0w
+”;
+
+val load_tcount_tm = “
+ s' with load_tcount := (s.fsm_state ≠ idle ∧ s.counter = 1w ∨ s.fsm_state = popFmtFifo)
+”;
+
+val log_start_tm = “
+ s' with log_start := (s.fsm_state = startSetupStart ∧ s.counter = 1w)
+”;
+
+val log_stop_tm = “
+ s' with log_stop := (s.fsm_state = stopClockStop ∧ s.counter = 1w)
+”;
+
+(* section --- FMT flags *)
+val fmt_fifo_rvalid_tm = “
+ s' with fmt_fifo := s'.fmt_fifo with rvalid := ¬s'.fmt_fifo.empty
+”;
+
+val fmt_fifo_flag_start_before_tm = “
+ s' with fmt_flag := s'.fmt_flag with start_before :=
+  (s'.fmt_fifo.rvalid ∧ word_bit 8 s'.fmt_fifo.rdata)
+”;
+
+val fmt_fifo_flag_stop_after_tm = “
+ s' with fmt_flag := s'.fmt_flag with stop_after :=
+ (s'.fmt_fifo.rvalid ∧ word_bit 9 s'.fmt_fifo.rdata)
+”;
+
+val fmt_fifo_flag_read_bytes_tm = “
+ s' with fmt_flag := s'.fmt_flag with read_bytes :=
+ (s'.fmt_fifo.rvalid ∧ word_bit 10 s'.fmt_fifo.rdata)
+”;
+
+val fmt_byte_tm = “
+ s' with fmt_byte :=
+ if s'.fmt_fifo.rvalid then (7 >< 0) s'.fmt_fifo.rdata else 0w
+”;
+
+val fmt_fifo_flag_nak_ok_tm = “
+ s' with fmt_flag := s'.fmt_flag with nak_ok := word_bit 12 s'.fmt_fifo.rdata
+”;
+
+val req_restart_tm = “
+ s' with req_restart := ( ¬s'.fmt_flag.read_bytes
+                        ∧  s'.fmt_flag.start_before
+                        ∧  s.fsm_state = active
+                        ∧  s.trans_started )
+”;
+
+val bit_clr_tm = “
+ s' with bit_clr := ( (s.fsm_state = transHoldBit ∨ s.fsm_state = recReadHoldBit)
+                    ∧  s.counter = 1w ∧ s.bit_index = 0w )
+”;
+
+val bit_decr_tm = “
+ s' with bit_decr := ((s.fsm_state = transHoldBit ∨ s.fsm_state = recReadHoldBit)
+                     ∧ s.counter = 1w ∧ s.bit_index ≠ 0w )
+”;
+
+val stretch_en_tm = “
+ s' with stretch_en := (s.fsm_state = transClockPulse
+                     ∨  s.fsm_state = transClockPulseAck
+                     ∨  s.fsm_state = recReadClockPulse
+                     ∨  s.fsm_state = recHostClockPulseAck)
+”;
+
+val scl_d_tm = “
+ s' with scl_d := ¬( s.fsm_state = startClockStart
+                   ∨ s.fsm_state = transClockLow
+                   ∨ s.fsm_state = transHoldBit
+                   ∨ s.fsm_state = transClockLowAck
+                   ∨ s.fsm_state = transHoldDevAck
+                   ∨ s.fsm_state = recReadClockLow
+                   ∨ s.fsm_state = recReadHoldBit
+                   ∨ s.fsm_state = recHostClockLowAck
+                   ∨ s.fsm_state = recHostHoldBitAck
+                   ∨ s.fsm_state = recHostHoldBitAck
+                   ∨ s.fsm_state = stopClockStop
+                   ∨ s.fsm_state = active ∧ (¬s'.fmt_flag.start_before ∨ s.trans_started)
+                   ∨ s.fsm_state = popFmtFifo ∧ ¬s'.fmt_flag.stop_after)
+”;
+
+val next_scl_rx_val_tm = “
+ if fext.cio_scl_i then
+   s' with next_scl_rx_val := (w2w s.scl_rx_val <<~ 1w) || 1w
+ else
+   s' with next_scl_rx_val := (w2w s.scl_rx_val <<~ 1w)
+”
+
+val next_stretch_idle_cnt_tm = “
+ if s'.stretch_en ∧ s'.scl_d ∧ ¬fext.cio_scl_i
+ then s' with next_stretch_idle_cnt := s.stretch_idle_cnt + 1w
+ else s' with next_stretch_idle_cnt := 0w
+”;
+
+val next_counter_tm = “
+ if s'.load_tcount then s' with next_counter := s'.curr_delay
+ else if s.stretch_idle_cnt = 0w then s' with next_counter := s.counter - 1w
+ else s' with next_counter := s.counter
+”;
+
+val byte_clr_tm = “
+ s' with byte_clr := (s.fsm_state = active ∧ s'.fmt_flag.read_bytes)
+”
+
+val byte_decr_tm= “
+ s' with byte_decr := (s.fsm_state = recHostHoldBitAck ∧ s.counter = 1w ∧ s.byte_index ≠ 1w)
+”
+
+val byte_num_tm = “
+ if s'.fmt_flag.read_bytes then s' with byte_num := 0w
+ else if s'.fmt_byte = 0w then s' with byte_num := 256w
+ else s' with byte_num := w2w s'.fmt_byte
+”
+
+val next_byte_index_tm = “
+ if s'.byte_clr then s' with next_byte_index := s'.byte_num
+ else if s'.byte_decr then s' with next_byte_index := s.byte_index - 1w
+ else s' with next_byte_index := s.byte_index
+”;
+
+val fifo_depth_tm = “
+     if s'.fmt_fifo.full then
+       s' with fmt_fifo := s'.fmt_fifo with depth := 64w
+     else if word_bit 6 s.fmt_fifo.wptr = word_bit 6 s.fmt_fifo.rptr then
+       s' with fmt_fifo := s'.fmt_fifo with depth := ((w2w ((5 >< 0) s.fmt_fifo.wptr : 6 word)) - (w2w ((5 >< 0) s.fmt_fifo.rptr : 6 word)))
+     else
+       s' with fmt_fifo := s'.fmt_fifo with depth := 64w - w2w ((5 >< 0) s.fmt_fifo.rptr : 6 word) + w2w ((5 >< 0) s.fmt_fifo.wptr :  6 word)
+”;
+
+val counter_gt_one_tm = “
+ s' with cnt_gt_one := (1w <+ s.counter)
+”;
+
+val next_state_tm = “
+  case s.fsm_state of
+    idle                 => if s.regs.ctrl.enablehost = 1w ∧ s'.fmt_fifo.rvalid
+                            then s' with next_state := active
+                            else s' with next_state := idle
+  | active               => if s'.fmt_flag.read_bytes then
+                              s' with next_state := recReadClockLow
+                            else if s'.fmt_flag.start_before ∧ ¬s.trans_started then
+                              s' with next_state := startSetupStart
+                            else
+                              s' with next_state := transClockLow
+
+  | recReadClockLow      => if s'.cnt_gt_one then s' with next_state := recReadClockLow
+                            else s' with next_state := recReadClockPulse
+
+  | recReadClockPulse    => if s'.cnt_gt_one then s' with next_state := recReadClockPulse
+                            else s' with next_state := recReadHoldBit
+
+  | recReadHoldBit       => if s'.cnt_gt_one then
+                              s' with next_state := recReadHoldBit
+                            else if s.bit_index = 0w then
+                              s' with next_state := recHostClockLowAck
+                            else
+                              s' with next_state := recReadClockLow
+
+  | recHostClockLowAck   => if s'.cnt_gt_one then s' with next_state := recHostClockLowAck
+                            else s' with next_state := recHostClockPulseAck
+
+  | recHostClockPulseAck => if s'.cnt_gt_one then s' with next_state := recHostClockPulseAck
+                            else s' with next_state := recHostHoldBitAck
+
+  | recHostHoldBitAck    => if s'.cnt_gt_one then
+                              s' with next_state := recHostHoldBitAck
+                            else if s.byte_index = 1w ∧ s'.fmt_flag.stop_after then
+                              s' with next_state := stopClockStop
+                            else if s.byte_index = 1w ∧ ¬s'.fmt_flag.stop_after then
+                              s' with next_state := popFmtFifo
+                            else
+                              s' with next_state := recReadClockLow
+
+  | stopClockStop        => if s'.cnt_gt_one then s' with next_state := stopClockStop
+                            else s' with next_state := stopSetupStop
+
+  | stopSetupStop        => if s'.cnt_gt_one then s' with next_state := stopSetupStop
+                            else s' with next_state := stopHoldStop
+
+  | stopHoldStop         => if s'.cnt_gt_one then s' with next_state := stopHoldStop
+                            else if s.regs.ctrl.enablehost = 0w then s' with next_state := idle
+                            else s' with next_state := popFmtFifo
+
+  | startSetupStart      => if s'.cnt_gt_one then s' with next_state := startSetupStart
+                            else s' with next_state := startHoldStart
+
+  | startHoldStart       => if s'.cnt_gt_one then s' with next_state := startHoldStart
+                            else s' with next_state := startClockStart
+
+  | startClockStart      => if s'.cnt_gt_one then s' with next_state := startClockStart
+                            else s' with next_state := transClockLow
+
+  | transClockLow        => if s'.cnt_gt_one then s' with next_state := transClockLow
+                            else if s.pend_restart then s' with next_state := startSetupStart
+                            else s' with next_state := transClockPulse
+
+  | transClockPulse      => if s'.cnt_gt_one then s' with next_state := transClockPulse
+                            else s' with next_state := transHoldBit
+
+  | transHoldBit         => if s'.cnt_gt_one then s' with next_state := transHoldBit
+                            else if s.bit_index = 0w then s' with next_state := transClockLowAck
+                            else s' with next_state := transClockLow
+
+  | transClockLowAck     => if s'.cnt_gt_one then s' with next_state := transClockLowAck
+                            else s' with next_state := transClockPulseAck
+
+  | transClockPulseAck   => if s'.cnt_gt_one then s' with next_state := transClockPulseAck
+                            else s' with next_state := transHoldDevAck
+
+  | transHoldDevAck      => if s'.cnt_gt_one then
+                              s' with next_state := transHoldDevAck
+                            else if s'.fmt_flag.stop_after then
+                              s' with next_state := stopClockStop
+                            else
+                              s' with next_state := popFmtFifo
+
+  | popFmtFifo           => if s.regs.ctrl.enablehost = 0w then s' with next_state := stopClockStop
+                            else if s'.fmt_fifo.depth = 1w then s' with next_state := idle
+                            else s' with next_state := active
+
+  | _ => s' with next_state := idle
+”;
+
+val read_byte_clr_tm = “
+ s' with read_byte_clr := (s.fsm_state = recReadHoldBit ∧ s.counter = 1w ∧ s.bit_index = 0w)
+”;
+
+val shift_data_en_tm = “
+ s' with shift_data_en := (s.fsm_state = recReadClockPulse ∧ s.counter = 1w)
+”;
+
+val next_sda_rx_val_tm = “
+ if fext.cio_sda_i then
+   s' with next_sda_rx_val := (w2w s.sda_rx_val <<~ 1w) || 1w
+ else
+   s' with next_sda_rx_val := (w2w s.sda_rx_val <<~ 1w)
+”;
+
+val next_read_byte_tm = “
+ if s'.read_byte_clr then s' with next_read_byte := 0w
+ else if s'.shift_data_en ∧ fext.cio_sda_i then
+   s' with next_read_byte := (w2w s.read_byte <<~ 1w) || 1w
+ else if s'.shift_data_en ∧ ¬fext.cio_sda_i then
+   s' with next_read_byte := (w2w s.read_byte <<~ 1w)
+ else
+   s' with next_read_byte := s.read_byte
+”;
+
+(* Section RX FIFO *)
+val rx_fifo_reset_tm = “
+ s' with rx_fifo := s'.rx_fifo with reset :=
+ (word_bit 0 s'.reg2hw.fifo_ctrl.rxrst_q ∧ s.reg2hw.fifo_ctrl.rxrst_qe)
+”;
+
+val rx_fifo_rdata_tm = “
+ s' with rx_fifo := s'.rx_fifo with rdata := s.rx_fifo_regfile $ (5 >< 0) s.rx_fifo.rptr
+”;
+
+val rx_fifo_rready_tm = “
+ s' with rx_fifo := s'.rx_fifo with rready := s'.reg2hw.rdata.rdata_re
+”;
+
+val rx_fifo_empty_tm = “
+ s' with rx_fifo := s'.rx_fifo with empty := (s.rx_fifo.rptr = s.rx_fifo.wptr)
+”;
+
+val rx_fifo_incr_rptr_tm = “
+ s' with rx_fifo := s'.rx_fifo with incr_rptr := (¬s'.rx_fifo.empty ∧ s'.rx_fifo.rready)
+”;
+
+val rx_fifo_counter_rptr_wrap_tm = “
+ s' with rx_fifo := s'.rx_fifo with counter := s'.rx_fifo.counter with rptr_wrap :=
+   (s'.rx_fifo.incr_rptr ∧ (5 >< 0) s.rx_fifo.rptr = 63w : 6 word)
+”;
+
+val rx_fifo_counter_rptr_wrap_cnt_tm = “
+ s' with rx_fifo := s'.rx_fifo with counter := s'.rx_fifo.counter with rptr_wrap_cnt :=
+  if ¬ word_bit 6 s.rx_fifo.rptr then (64w : 7 word) else 0w
+”;
+
+val rx_fifo_rptr_tm = “
+ if s'.rx_fifo.reset then
+   s' with rx_fifo := s'.rx_fifo with rptr := 0w
+ else if s'.rx_fifo.counter.rptr_wrap then
+   s' with rx_fifo := s'.rx_fifo with rptr := s'.rx_fifo.counter.rptr_wrap_cnt
+ else
+   s' with rx_fifo := s'.rx_fifo with rptr := s.rx_fifo.rptr + 1w
+”;
+
+val rx_fifo_wvalid_tm = “
+ s' with rx_fifo := s'.rx_fifo with wvalid :=
+ (s.fsm_state = recReadHoldBit ∧ s.bit_index = 0w ∧ s.counter = 1w)
+”;
+
+val rx_fifo_wdata_tm = “
+ if s.fsm_state = recReadHoldBit ∧ s.bit_index = 0w ∧ s.counter = 1w then
+   s' with rx_fifo := s'.rx_fifo with wdata := s.read_byte
+ else
+   s' with rx_fifo := s'.rx_fifo with wdata := 0w
+”;
+
+val rx_fifo_full_tm = “
+ s' with rx_fifo := s'.rx_fifo with full :=
+   ((word_bit 5 s.rx_fifo.wptr ≠ word_bit 5 s.rx_fifo.rptr) ∧
+   ((5 >< 0) s.rx_fifo.wptr : 6 word = (5 >< 0) s.rx_fifo.rptr : 6 word))
+”;
+
+val rx_fifo_incr_wptr_tm = “
+ s' with rx_fifo := s'.rx_fifo with incr_wptr := (¬s'.rx_fifo.full ∧ s'.rx_fifo.wvalid)
+”;
+
+val rx_fifo_regfile_tm = “
+ let
+   wptr = (5 >< 0) s.rx_fifo.wptr;
+ in
+   if s'.rx_fifo.incr_wptr
+   then s' with rx_fifo_regfile := (wptr =+ s'.rx_fifo.wdata) s'.rx_fifo_regfile
+   else s'
+”;
+
+val rx_fifo_counter_wptr_wrap_tm = “
+ s' with rx_fifo := s'.rx_fifo with counter := s'.rx_fifo.counter with wptr_wrap :=
+   (s'.rx_fifo.incr_wptr ∧ (5 >< 0) s.rx_fifo.wptr = 63w : 6 word)
+”;
+
+val rx_fifo_counter_wptr_wrap_cnt_tm = “
+ s' with rx_fifo := s'.rx_fifo with counter := s'.rx_fifo.counter with wptr_wrap_cnt :=
+  if ¬word_bit 6 s.rx_fifo.wptr then 64w else 0w
+”;
+
+val rx_fifo_wptr_tm = “
+ if s'.rx_fifo.reset then
+   s' with rx_fifo := s'.rx_fifo with wptr := 0w
+ else if s'.rx_fifo.counter.wptr_wrap then
+   s' with rx_fifo := s'.rx_fifo with wptr := s'.rx_fifo.counter.wptr_wrap_cnt
+ else
+   s' with rx_fifo := s'.rx_fifo with wptr := s.rx_fifo.wptr + 1w
+”;
+
+val hw2reg_intr_state_nak_de_tm = “
+ s' with hw2reg := s'.hw2reg with intr_state := s'.hw2reg.intr_state with nak_de :=
+ (s.fsm_state = transClockPulseAck ∧ ¬s'.fmt_flag.nak_ok ∧ fext.cio_sda_i)
+”;
+
+val hw2reg_intr_state_nak_d_tm = “
+ s' with hw2reg := s'.hw2reg with intr_state := s'.hw2reg.intr_state with nak_d :=
+ n2w $ bool_to_bit
+     ( s.fsm_state = transClockPulseAck ∧ ¬s'.fmt_flag.nak_ok ∧ fext.cio_sda_i
+     ∨ word_bit 0 s'.reg2hw.intr_state.nak_q)
+”;
+
+val next_intr_nak_o_tm = “
+ s' with next_intr_nak_o := (word_bit 0 s'.reg2hw.intr_state.nak_q ∧ word_bit 0 s'.reg2hw.intr_enable.nak_q)
+”
+
+val hw2reg_intr_state_cmd_complete_de_tm = “
+ s' with hw2reg := s'.hw2reg with intr_state := s'.hw2reg.intr_state with cmd_complete_de :=
+ (s.fsm_state = stopHoldStop ∨ s.fsm_state = startSetupStart ∧ s'.log_start ∧ s.pend_restart)
+”;
+
+val hw2reg_intr_state_cmd_complete_d_tm = “
+ s' with hw2reg := s'.hw2reg with intr_state := s'.hw2reg.intr_state with cmd_complete_d :=
+ if ( s.fsm_state = stopHoldStop ∨ s.fsm_state = startSetupStart ∧ s'.log_start ∧ s.pend_restart
+ ∨ word_bit 0 s'.reg2hw.intr_state.cmd_complete_q ) then 1w else 0w
+”
+
+val next_intr_cmd_complete_o_tm = “
+ s' with next_intr_cmd_complete_o := (word_bit 0 s'.reg2hw.intr_state.cmd_complete_q ∧ word_bit 0 s'.reg2hw.intr_enable.cmd_complete_q)
+”;
+
+val next_pend_restart_tm = “
+ if s.pend_restart ∧ s.regs.ctrl.enablehost = 0w ∨ s'.log_start then s' with next_pend_restart := F
+ else if s'.req_restart then s' with next_pend_restart := T
+ else s' with next_pend_restart := s.pend_restart
+”;
+
+val next_trans_started_tm = “
+ if s.trans_started ∧ s.regs.ctrl.enablehost = 0w ∨ s'.log_stop then s' with next_trans_started := F
+ else if s'.log_start then s' with next_trans_started := T
+ else s' with next_trans_started := s.trans_started
+”;
+
+val next_bit_index_tm = “
+ if s'.bit_clr then s' with next_bit_index := 7w
+ else if s'.bit_decr then s' with next_bit_index := s.bit_index - 1w
+ else s' with next_bit_index := s.bit_index
+”;
+
+val i2c_core_ff_tm = “
+  s' with fsm_state := s'.next_state
+”;
+
+val i2c_core_counter_ff_tm = “
+  s' with counter := s'.next_counter
+”;
+
+val i2c_core_stretch_idle_cnt_ff_tm = “
+  s' with stretch_idle_cnt := s'.next_stretch_idle_cnt
+”;
+
+val bit_index_ff_tm = “
+  s' with bit_index := s'.next_bit_index
+”;
+
+val pend_restart_ff_tm = “
+  s' with pend_restart := s'.next_pend_restart
+”;
+
+val byte_index_ff_tm = “
+  s' with byte_index := s'.next_byte_index
+”;
+
+end
