i2c/i2cCircuitCompileScript.sml
@@ -5,6 +5,52 @@ open i2cCircuitTheory;
 
 val _ = new_theory "i2cCircuitCompile";
 
+Theorem i2c_circuit_alt_def:
+i2c_circuit =
+     mk_module
+       (procs
+          ([i2c_core_counter_ff; i2c_core_stretch_idle_cnt_ff;
+            fmt_fifo_rptr_ff; fmt_fifo_regfile_ff; i2c_core_rx_fifo_wptr_ff;
+            fmt_fifo_wptr_ff; bit_index_ff; pend_restart_ff; byte_index_ff;
+            i2c_core_rx_fifo_rptr_ff; i2c_core_rx_fifo_regfile; i2c_core_ff;
+            i2c_reg_top_ff]))
+       (procs
+          ([i2c_reg_top_comb_1; i2c_core_rx_fifo_counter_wptr_wrap_comb;
+            i2c_core_rx_fifo_counter_wptr_wrap_cnt_comb; i2c_core_delay_comb;
+            i2c_core_curr_delay_comb; i2c_core_load_tcount_comb;
+            i2c_core_stretch_en_comb; i2c_core_scl_d_comb;
+            i2c_core_next_stretch_idle_cnt; i2c_core_next_counter;
+            i2c_core_next_state; fmt_fifo_reset; counter_gt_one_comb;
+            fmt_fifo_rdata; fmt_fifo_rready; fmt_fifo_empty;
+            fmt_fifo_counter_rptr_wrap; fmt_fifo_counter_rptr_wrap_cnt;
+            fmt_fifo_wvalid; fmt_fifo_full; fmt_fifo_incr_wptr;
+            fmt_fifo_wdata; fmt_fifo_counter_wptr_wrap;
+            fmt_fifo_counter_wptr_wrap_cnt; i2c_core_log_start_comb;
+            i2c_core_log_stop_comb; fmt_fifo_rvalid;
+            fmt_fifo_flag_start_before; fmt_fifo_flag_stop_after;
+            fmt_fifo_flag_read_bytes; fmt_byte; req_restart; bit_clr;
+            bit_decr; i2c_core_next_scl_rx_val_comb; i2c_core_byte_clr_comb;
+            i2c_core_byte_num_comb; i2c_core_next_byte_index_comb;
+            fifo_depth; i2c_core_read_byte_clr_comb;
+            i2c_core_shift_data_en_comb; i2c_core_next_sda_rx_val_comb;
+            i2c_core_next_read_byte_comb; i2c_core_rx_fifo_reset_comb;
+            i2c_core_rx_fifo_rdata_comb; i2c_core_rx_fifo_rready_comb;
+            i2c_core_rx_fifo_empty_comb; i2c_core_rx_fifo_incr_rptr_comb;
+            i2c_core_rx_fifo_counter_rptr_wrap_comb;
+            i2c_core_rx_fifo_counter_rptr_wrap_cnt_comb;
+            i2c_core_rx_fifo_wvalid_comb; i2c_core_rx_fifo_wdata_comb;
+            i2c_core_rx_fifo_full_comb; i2c_core_rx_fifo_incr_wptr_comb;
+            hw2reg_intr_state_nak_de_comb; next_intr_nak_comb;
+            hw2reg_intr_state_cmd_complete_de_comb;
+            hw2reg_intr_state_cmd_complete_d_comb;
+            next_intr_cmd_complete_comb; next_pend_restart_comb;
+            next_trans_started_comb; next_bit_index_comb;
+            i2c_reg_top_comb_2]))
+       i2c_circuit_init
+Proof
+  rw [i2c_circuit_def, i2c_core_ffs1_def, i2c_core_combs_def]
+QED
+
 local
   val outputs = [
     "reg_rsp_o",
@@ -31,8 +77,12 @@ local
     "intr_host_timeout_o"
   ];
   val comms = i2c_reg_comms @ [];
+  val comms = i2c_reg_comms @ ["fsm_state", "counter", "stretch_idle_cnt", "fmt_fifo_rptr", "fmt_fifo_wptr", "fmt_fifo_regfile",
+                             "rx_fifo_regfile", "rx_fifo_rptr", "rx_fifo_wptr", "bit_index", "pend_restart", "byte_index", "trans_started",
+                             "read_byte", "sda_rx_val", "scl_rx_val"]
+
 in
-  val tstate = init_translator i2c_circuit_def [] comms;
+  val tstate = init_translator i2c_circuit_alt_def [] comms;
   val trans_thm = module2hardware tstate i2c_circuit_def [] outputs comms;
 end
 
