i2c/i2cRegsCircuitProofScript.sml
@@ -1009,4 +1009,53 @@ Proof
   >> simp []
 QED
 
+val asm1_simp = BETA_RULE o REWRITE_RULE [combinTheory.C_THM, listTheory.EVERY_MEM] o GEN_ALL
+
+val ff_asm1' = ff_asm1 |> asm1_simp
+val comb_asm1' = comb_asm1 |> asm1_simp
+
+Theorem asm1:
+∀proc fext s s'.
+  MEM proc (i2c_core_ffs1 ++ [] ++ i2c_core_combs) ⇒
+  (let
+     s'' = proc fext s s'
+   in
+     s''.reg2hw = s'.reg2hw ∧ s''.regs = s'.regs ∧
+     s''.reg_rsp_o = s'.reg_rsp_o ∧ s''.addr = s'.addr ∧
+     (s''.write ⇔ s'.write) ∧ s''.wdata = s'.wdata ∧
+     s''.wstrb = s'.wstrb ∧ (s''.valid ⇔ s'.valid))
+Proof
+  ASSUME_TAC ff_asm1'
+  >> ASSUME_TAC comb_asm1'
+  >> rpt GEN_TAC
+  >> REWRITE_TAC [rich_listTheory.IS_EL_APPEND, listTheory.MEM]
+  >> STRIP_TAC
+  >> FIRST_X_ASSUM (fn th1 => FIRST_ASSUM (fn th2 => MATCH_MP th2 th1 |> REWRITE_RULE [LET_THM] |> BETA_RULE |> ASSUME_TAC))
+  >> rw [LET_THM]
+QED
+
+Theorem asm2:
+∀proc fext s s'. MEM proc i2c_core_ffs1 ⇒ (proc fext s s').hw2reg = s'.hw2reg
+Proof
+  rw [ff_asm2 |> asm1_simp]
+QED
+
+val _ = type_abbrev(
+  "proc_ty",
+  “:(i2c_circuit_ext_state -> i2c_circuit_state -> i2c_circuit_state -> i2c_circuit_state) list”);
+
+val i2c_reg_top_correct' = i2c_reg_top_correct
+             |> INST [“combs:proc_ty” |-> “i2c_core_combs” ,
+                      “ffs2:proc_ty” |-> “[]:proc_ty” ,
+                      “ffs1:proc_ty” |-> “i2c_core_ffs1”]
+             |> REWRITE_RULE [GSYM i2c_circuit_def, Ntimes LET_THM 1]
+             |> BETA_RULE
+             |> IMP_CANON
+             |> hd
+
+(* this is the theorem ‘i2c_reg_top_correct’ with the first two assumptions
+   being discharged, targetted specifically for ‘i2c_circuit’ *)
+val i2c_reg_top_correct_inst =
+  MATCH_MP (MATCH_MP i2c_reg_top_correct' asm1) asm2
+
 val _ = export_theory ();
